Update Dutch_National_Flag_Monad.thy
Updated structure of definitions and updated proofs

Monad_Play Around/DNFP/Dutch_National_Flag_Monad.thy
@@ -113,8 +113,9 @@ do{
  }))
 }"
 
+
+
 text\<open>A version using a state monad for storing the list/array that is being sorted\<close>
-(*\<comment> l < high \<and> i < h*)
 fun dnfp_mon:: "nat \<Rightarrow> (env, unit) state" where
 "dnfp_mon 0  = skip"|
 "dnfp_mon (Suc 0)  = skip"|
@@ -136,7 +137,7 @@ definition init_state_env:: "nat array \<Rightarrow> (env, unit) state" where
 
 definition mk_rec:: "nat array \<Rightarrow>nat \<Rightarrow> nat \<Rightarrow> nat \<Rightarrow> env" where
 "mk_rec arr l j h \<equiv> \<lparr>high = h,            low = l,
-                     i = j,                xs = arr\<rparr>"
+                     i = j,               xs = arr\<rparr>"
 
 value \<open>snd(run_state (dnfp_mon 5) (init_env [0,2,2,1,2]))\<close>
 value \<open>snd(run_state (dnfp_mon 9) (init_env [0,2,2,0,1,0,2,1,2]))\<close>
@@ -168,6 +169,10 @@ text\<open>This can be used in the other pre and post-conditions for the methods
 subsection\<open>Pre- and Postconditions\<close>
 
 subsubsection\<open>Pre-conditions\<close>
+definition dnfp_pre where
+"dnfp_pre e \<equiv> high e \<ge> i e
+              \<and> i e \<ge> low e 
+              \<and> length (xs e) \<ge> high e"
 
 definition init_loop_pre where
 "init_loop_pre e \<equiv> high e > i e 
@@ -175,8 +180,7 @@ definition init_loop_pre where
 
 
 definition loop_update_action_pre where
-"loop_update_action_pre e \<equiv> high e > i e 
-                              \<and> length (xs e) > (Suc 0)
+"loop_update_action_pre e \<equiv> init_loop_pre e
                               \<and> length (xs e) \<ge> high e
                               \<and> low e < high e
                               \<and> low e \<le> i e"
@@ -201,6 +205,10 @@ definition inc_index_pre where
 "inc_index_pre arr l j h \<equiv> loop_update_action_pre (mk_rec arr l j h) 
                               \<and> arr!j = 1"
 
+definition dnfp_pre_aux where
+"dnfp_pre_aux e \<equiv> 
+    (Suc 0)  < length (xs e) \<longrightarrow> (inc_index_pre (xs e) (low e) (i e) (high e) \<or> dec_highbound_pre (xs e) (low e) (i e) (high e) \<or> inc_lowbound_pre (xs e) (low e) (i e) (high e)) "
+
 subsubsection\<open>Post-conditions\<close>
 definition init_loop_post where 
 "init_loop_post e e'\<equiv> e = e'"
@@ -219,40 +227,37 @@ definition dec_highbound_post where
                               \<and> (xs e')!(high e') = 2
                               \<and> loop_update_action_post e e'"
 
-definition add_high_post where 
-"add_high_post e e' \<equiv> high e = high e' 
-                       \<and> low e = low e'
-                       \<and> i e = i e'
-                       \<and> length (xs e) = length (xs e')
-                       \<and> invariants (xs e') (low e') (i e') (high e')"
-
 definition inc_index_post where 
 "inc_index_post e e' \<equiv> high e = high e' 
                       \<and> low e = low e'
                       \<and> Suc(i e) = i e'
                       \<and> loop_update_action_post e e'"
 
+definition dnfp_post where 
+"dnfp_post e e2 \<equiv> length (xs e) = length (xs e2)
+                  \<and> length (xs e) > (Suc 0) \<longrightarrow> (inc_index_post e e2  \<or> dec_highbound_post e e2 \<or> inc_lowbound_post e e2)"
+
 section\<open>Lemmators\<close>
 subsection\<open>Inc_lowbound Invariants\<close>
 text\<open>Pre and post-condition\<close>
 lemma inc_lowbound_prepost: "\<lbrakk>inc_lowbound_pre arr l j h; (mk_rec arr l j h) = e; low_invariant_is_0 arr l;snd(run_state (inc_lowbound arr j) e) = e2 \<rbrakk> \<Longrightarrow> inc_lowbound_post e e2"
-  apply(simp_all add: inc_lowbound_pre_def mk_rec_def loop_update_action_pre_def inc_lowbound_post_def snd_def loop_update_action_post_def inc_lowbound_def)
+  apply(simp_all add: inc_lowbound_pre_def init_loop_pre_def mk_rec_def loop_update_action_pre_def inc_lowbound_post_def snd_def loop_update_action_post_def inc_lowbound_def)
   apply(simp_all add: put_xs_def get_low_def put_i_def swap_def return_def get_def put_def put_low_def set_low_def set_i_def set_xs_def)
   by(auto)
 
 subsubsection\<open>Invariants\<close>
 lemma inc_lowbound_invariantRed: "\<lbrakk>inc_lowbound_pre arr l j h; (mk_rec arr l j h) = e; low_invariant_is_0 (xs e) (low e);snd(run_state (inc_lowbound arr j) e) = e2 \<rbrakk> \<Longrightarrow> low_invariant_is_0 (xs e2) (low e2)"
-apply(simp_all add: inc_lowbound_pre_def mk_rec_def loop_update_action_pre_def low_invariant_is_0_def snd_def loop_update_action_post_def inc_lowbound_def)
+apply(simp_all add: inc_lowbound_pre_def init_loop_pre_def mk_rec_def loop_update_action_pre_def low_invariant_is_0_def snd_def loop_update_action_post_def inc_lowbound_def)
   apply(simp_all add: put_xs_def get_low_def put_i_def swap_def return_def get_def put_def put_low_def set_low_def set_i_def set_xs_def)
   using less_Suc_eq by (auto)
 
 lemma inc_lowbound_invariantBlue: "\<lbrakk>inc_lowbound_pre arr l j h; (mk_rec arr l j h) = e; high_invariant_is_2 (xs e) (high e);snd(run_state (inc_lowbound arr j) e) = e2 \<rbrakk> \<Longrightarrow> high_invariant_is_2 (xs e2) (high e2)"
-apply(simp_all add: inc_lowbound_pre_def mk_rec_def loop_update_action_pre_def high_invariant_is_2_def snd_def loop_update_action_post_def inc_lowbound_def)
+apply(simp_all add: inc_lowbound_pre_def init_loop_pre_def mk_rec_def loop_update_action_pre_def high_invariant_is_2_def snd_def loop_update_action_post_def inc_lowbound_def)
   apply(simp_all add: put_xs_def get_low_def put_i_def swap_def return_def get_def put_def put_low_def set_low_def set_i_def set_xs_def)
   using less_Suc_eq by (auto)
 
 lemma inc_lowbound_invariantWhite: "\<lbrakk>inc_lowbound_pre arr l j h; (mk_rec arr l j h) = e; invariant_low_to_j_is_1 (xs e) (low e) (i e);snd(run_state (inc_lowbound arr j) e) = e2 \<rbrakk> \<Longrightarrow> invariant_low_to_j_is_1 (xs e2) (low e2) (i e2)"
-apply(simp_all add: inc_lowbound_pre_def mk_rec_def loop_update_action_pre_def invariant_low_to_j_is_1_def snd_def loop_update_action_post_def inc_lowbound_def)
+apply(simp_all add: inc_lowbound_pre_def init_loop_pre_def mk_rec_def loop_update_action_pre_def invariant_low_to_j_is_1_def snd_def loop_update_action_post_def inc_lowbound_def)
   apply(simp_all add: put_xs_def get_low_def put_i_def swap_def return_def get_def put_def put_low_def set_low_def set_i_def set_xs_def)
   using less_Suc_eq by (auto)
 
@@ -262,7 +267,7 @@ lemma inc_lowbound_inv: "\<lbrakk>inc_lowbound_pre arr l j h; (mk_rec arr l j h)
 
 subsection\<open>Dec_highbound Invariants\<close>
 lemma dec_highbound_prepost[simp]: "\<lbrakk>dec_highbound_pre arr l j h; (mk_rec arr l j h) = e; snd(run_state (dec_highbound arr j h) e) = e2 \<rbrakk> \<Longrightarrow> dec_highbound_post e e2"
-  apply(simp_all add: dec_highbound_pre_def mk_rec_def loop_update_action_pre_def dec_highbound_post_def snd_def loop_update_action_post_def dec_highbound_def)
+  apply(simp_all add: dec_highbound_pre_def init_loop_pre_def mk_rec_def loop_update_action_pre_def dec_highbound_post_def snd_def loop_update_action_post_def dec_highbound_def)
   apply(simp_all add: put_high_def add_high_def set_high_def put_xs_def put_def get_def swap_def set_xs_def)
   by(auto)
 
@@ -273,12 +278,12 @@ apply(simp_all add: dec_highbound_pre_def mk_rec_def loop_update_action_pre_def 
   by (auto)
 
 lemma dec_highbound_invariantWhite: "\<lbrakk>dec_highbound_pre arr l j h; (mk_rec arr l j h) = e; invariant_low_to_j_is_1 (xs e) (low e) (i e);snd(run_state (dec_highbound arr j h) e) = e2 \<rbrakk> \<Longrightarrow> invariant_low_to_j_is_1 (xs e2) (low e2) (i e2)"
-apply(simp_all add: dec_highbound_pre_def mk_rec_def loop_update_action_pre_def invariant_low_to_j_is_1_def snd_def loop_update_action_post_def dec_highbound_def)
+apply(simp_all add: dec_highbound_pre_def init_loop_pre_def mk_rec_def loop_update_action_pre_def invariant_low_to_j_is_1_def snd_def loop_update_action_post_def dec_highbound_def)
   apply(simp_all add: put_high_def add_high_def set_high_def put_xs_def put_def get_def swap_def set_xs_def)
   by (auto)
 
 lemma dec_highbound_invariantBlue: "\<lbrakk>dec_highbound_pre arr l j h; (mk_rec arr l j h) = e; high_invariant_is_2 (xs e) (high e);snd(run_state (dec_highbound arr j h) e) = e2 \<rbrakk> \<Longrightarrow> high_invariant_is_2 (xs e2) (high e2)"
-apply(simp_all add: dec_highbound_pre_def mk_rec_def loop_update_action_pre_def high_invariant_is_2_def snd_def loop_update_action_post_def dec_highbound_def)
+apply(simp_all add: dec_highbound_pre_def init_loop_pre_def mk_rec_def loop_update_action_pre_def high_invariant_is_2_def snd_def loop_update_action_post_def dec_highbound_def)
   apply(simp_all add: put_high_def add_high_def set_high_def put_xs_def put_def get_def swap_def set_xs_def)
   by (smt Suc_pred le_less_Suc_eq length_list_update not_less not_less_eq nth_list_update nth_list_update_neq select_convs(1) select_convs(4) zero_less_Suc)
 
@@ -288,7 +293,7 @@ lemma dec_highbound_inv: "\<lbrakk>dec_highbound_pre arr l j h; (mk_rec arr l j 
 
 subsection\<open>Inc_index Invariants\<close>
 lemma inc_index_prepost: "\<lbrakk>inc_index_pre arr l j h;  (mk_rec arr l j h) = e; snd(run_state (inc_index j) e) = e2\<rbrakk> \<Longrightarrow> inc_index_post e e2"
-  apply(simp_all add: snd_def mk_rec_def inc_index_def inc_index_post_def inc_index_pre_def loop_update_action_pre_def loop_update_action_post_def)
+  apply(simp_all add: snd_def mk_rec_def init_loop_pre_def inc_index_def inc_index_post_def inc_index_pre_def loop_update_action_pre_def loop_update_action_post_def)
   apply(simp_all add: invariants_def low_invariant_is_0_def invariant_low_to_j_is_1_def high_invariant_is_2_def put_i_def get_def set_i_def put_def)
   by (auto)
 
@@ -314,49 +319,46 @@ lemma inc_index_inv: "\<lbrakk>inc_index_pre arr l j h; (mk_rec arr l j h) = e; 
 
 subsection\<open>Loop update action\<close>
 lemma loop_update_action_prepost: "\<lbrakk>(mk_rec arr l j h) = e; loop_update_action_pre e; snd(run_state (loop_update_action arr j h) e) = e2 \<rbrakk> \<Longrightarrow> loop_update_action_post e e2"
-  apply(simp_all add:  mk_rec_def loop_update_action_pre_def snd_def loop_update_action_post_def loop_update_action_def)
+  apply(simp_all add:  mk_rec_def loop_update_action_pre_def init_loop_pre_def snd_def loop_update_action_post_def loop_update_action_def)
   apply(simp_all only: inc_lowbound_def dec_highbound_def inc_index_def get_low_def put_high_def set_high_def put_xs_def put_def get_def swap_def)
   apply(simp_all only: set_low_def put_low_def set_xs_def put_i_def add_high_def put_def get_def set_i_def put_xs_def swap_def)
   apply(simp only: return_def)
   by(auto)
 
 subsubsection\<open>Invariants\<close>
+lemma  loop_update_action_invariantRed: "\<lbrakk>(mk_rec arr l j h) = e; loop_update_action_pre e; inc_lowbound_pre arr l j h \<or> dec_highbound_pre arr l j h \<or> inc_index_pre arr l j h; low_invariant_is_0 (xs e) (low e);snd(run_state (loop_update_action arr j h) e) = e2 \<rbrakk> \<Longrightarrow> low_invariant_is_0 (xs e2) (low e2)"
+  using dec_highbound_invariantRed inc_index_invariantRed inc_index_pre_def inc_lowbound_invariantRed inc_lowbound_pre_def loop_update_action_def by fastforce
 
-text\<open>I think I should be able to use the lemmators defined above\<close>
-lemma  loop_update_action_invariantRed: "\<lbrakk>(mk_rec arr l j h) = e; loop_update_action_pre e;  low_invariant_is_0 (xs e) (low e);snd(run_state (loop_update_action arr j h) e) = e2 \<rbrakk> \<Longrightarrow> low_invariant_is_0 (xs e2) (low e2)"
-  apply(simp_all add: mk_rec_def loop_update_action_pre_def low_invariant_is_0_def snd_def loop_update_action_post_def loop_update_action_def)
-  apply(simp_all only: inc_lowbound_def dec_highbound_def inc_index_def get_low_def put_high_def set_high_def put_xs_def put_def get_def swap_def)
-   apply(simp_all only: set_low_def put_low_def set_xs_def put_i_def add_high_def put_def get_def set_i_def put_xs_def swap_def return_def)
-  sorry
+lemma  loop_update_action_invariantBlue: "\<lbrakk>(mk_rec arr l j h) = e; loop_update_action_pre e; inc_lowbound_pre arr l j h \<or> dec_highbound_pre arr l j h \<or> inc_index_pre arr l j h;  high_invariant_is_2 (xs e) (high e);snd(run_state (loop_update_action arr j h) e) = e2 \<rbrakk> \<Longrightarrow> high_invariant_is_2 (xs e2) (high e2)"
+  using dec_highbound_invariantBlue inc_index_invariantBlue inc_index_pre_def inc_lowbound_invariantBlue inc_lowbound_pre_def loop_update_action_def by fastforce
 
-lemma  loop_update_action_invariantBlue: "\<lbrakk>(mk_rec arr l j h) = e; loop_update_action_pre e;  high_invariant_is_2 (xs e) (high e);snd(run_state (loop_update_action arr j h) e) = e2 \<rbrakk> \<Longrightarrow> high_invariant_is_2 (xs e2) (high e2)"
-apply(simp_all add: mk_rec_def loop_update_action_pre_def high_invariant_is_2_def snd_def loop_update_action_post_def loop_update_action_def)
-  apply(simp_all only: inc_lowbound_def dec_highbound_def inc_index_def get_low_def put_high_def set_high_def put_xs_def put_def get_def swap_def)
-  apply(simp_all only: set_low_def put_low_def set_xs_def put_i_def add_high_def put_def get_def set_i_def put_xs_def swap_def)
-  apply(simp only: return_def)
-  sorry
-
-lemma  loop_update_action_invariantWhite: "\<lbrakk>(mk_rec arr l j h) = e; loop_update_action_pre e;  invariant_low_to_j_is_1 (xs e) (low e) (i e);snd(run_state (loop_update_action arr j h) e) = e2 \<rbrakk> \<Longrightarrow> invariant_low_to_j_is_1 (xs e2) (low e2) (i e2)"
-apply(simp_all add: mk_rec_def loop_update_action_pre_def invariant_low_to_j_is_1_def snd_def loop_update_action_post_def loop_update_action_def)
-  apply(simp_all only: inc_lowbound_def dec_highbound_def inc_index_def get_low_def put_high_def set_high_def put_xs_def put_def get_def swap_def)
-   apply(simp_all only: set_low_def put_low_def set_xs_def put_i_def add_high_def put_def get_def set_i_def put_xs_def swap_def)
-  apply(simp only: return_def)
-  sorry
-
+lemma  loop_update_action_invariantWhite: "\<lbrakk>(mk_rec arr l j h) = e; loop_update_action_pre e; inc_lowbound_pre arr l j h \<or> dec_highbound_pre arr l j h \<or> inc_index_pre arr l j h; invariant_low_to_j_is_1 (xs e) (low e) (i e);snd(run_state (loop_update_action arr j h) e) = e2 \<rbrakk> \<Longrightarrow> invariant_low_to_j_is_1 (xs e2) (low e2) (i e2)"
+  using dec_highbound_invariantWhite inc_index_invariantWhite inc_index_pre_def inc_lowbound_invariantWhite inc_lowbound_pre_def loop_update_action_def by fastforce
 
 text\<open>The difference between high and i will never increase and will be decreased by loop_update_action\<close>
 lemma termination_loop_update_action:
 "\<lbrakk>(mk_rec arr l j h) = e; loop_update_action_pre e; snd(run_state (loop_update_action arr j h) e) = e2 \<rbrakk> \<Longrightarrow> (high e2 - i e2) < (high e - i e)"
   using loop_update_action_post_def loop_update_action_prepost by blast
 
-
 subsection\<open>Init_loop\<close>
 lemma init_loop_prepost: "\<lbrakk>init_loop_pre e; snd(run_state (init_loop) e) = e2\<rbrakk> \<Longrightarrow> init_loop_post e e2"
   by(simp_all add: init_loop_pre_def snd_def init_loop_def init_loop_post_def get_xs_def get_i_def get_def get_high_def return_def)
 
 subsubsection\<open>Invariants\<close>
+text\<open>This is a very since proof since the method does not change any state at all\<close>
 lemma init_loop_inv: "\<lbrakk>init_loop_pre e; invariant_low_to_j_is_1 (xs e) (low e) (i e); high_invariant_is_2 (xs e) (high e);
                         low_invariant_is_0 (xs e) (low e); snd(run_state (init_loop) e) = e2 \<rbrakk> \<Longrightarrow> invariant_low_to_j_is_1 (xs e2) (low e2) (i e2) \<and> low_invariant_is_0 (xs e2) (low e2) \<and> high_invariant_is_2 (xs e2) (high e2)"
   by (metis init_loop_post_def init_loop_prepost)
+
+subsection\<open>DNFP proof\<close>
+lemma dnfp_prepost: "\<lbrakk>(mk_rec arr l j h) = e; dnfp_pre e; dnfp_pre_aux e; length arr = n; snd(run_state (dnfp_mon n) e) = e2 \<rbrakk> \<Longrightarrow> dnfp_post e e2"
+  apply(simp_all add:  dnfp_pre_def dnfp_pre_aux_def snd_def dnfp_post_def high_invariant_is_2_def loop_update_action_post_def)
+  apply(simp_all add: inc_lowbound_pre_def inc_index_pre_def loop_update_action_pre_def mk_rec_def init_loop_pre_def dec_highbound_pre_def)
+  apply(simp_all add: inc_lowbound_post_def inc_index_post_def loop_update_action_post_def dec_highbound_post_def)
+  apply(induction n rule:dnfp_mon.induct)
+   apply force
+   apply force
+  sledgehammer
+  sorry
 
 end
